actually add new proofs

deps/poulet4/lib/P4automata/Benchmarks/EnterpriseSelfProof.v
@@ -22,40 +22,6 @@ Definition r_states : list (Reachability.state_pair A) :=
                         start_right).
 
 
-
-(* Definition r_states' :=
-  Eval vm_compute in (Reachability.reachable_step r_states).
-
-Definition r_len := Eval vm_compute in (length r_states, length r_states').
-
-Print r_len. *)
-
-Definition top : Relations.rel conf := fun _ _ => True.
-Definition top' : Relations.rel (state_template A) := fun _ _ => True.
-
-ClearEnvCtors.
-
-(* | HdrEth: header eth_size
-| HdrVLAN0: header vlan_size
-| HdrVLAN1: header vlan_size
-| HdrIPv4: header ipv4_size
-| HdrIPv6: header ipv6_size
-| HdrTCP: header tcp_size
-| HdrUDP: header udp_size
-| HdrICMP *)
-
-(*
-RegisterEnvCtors
-  (Enterprise.HdrEth, FirstOrderConfRelSimplified.Bits eth_size)
-  (Enterprise.HdrVLAN0, FirstOrderConfRelSimplified.Bits vlan_size)
-  (Enterprise.HdrVLAN1, FirstOrderConfRelSimplified.Bits vlan_size)
-  (Enterprise.HdrIPv4, FirstOrderConfRelSimplified.Bits ipv4_size)
-  (Enterprise.HdrIPv6, FirstOrderConfRelSimplified.Bits ipv6_size)
-  (Enterprise.HdrTCP, FirstOrderConfRelSimplified.Bits tcp_size)
-  (Enterprise.HdrUDP, FirstOrderConfRelSimplified.Bits udp_size)
-  (Enterprise.HdrICMP, FirstOrderConfRelSimplified.Bits icmp_size).
-*)
-
 Lemma prebisim_babyip:
   forall q1 q2,
     interp_conf_rel' {| cr_st := {|
